Changed relations in WellScoped.v, and derived checkers/proofs for these relations

src/Language/PlutusIR/Analysis/WellScoped.v
@@ -14,13 +14,8 @@ From QuickChick Require Import QuickChick.
 
 Definition ctx := list string.
 
-Definition tvd_name (tvd : tvdecl tyname) : tyname :=
-  match tvd with
-  | TyVarDecl v K => v
-  end.
-
 Reserved Notation "Δ '|-*' T" (at level 40, T at level 0).
-Inductive well_scoped_Ty (Δ : ctx) : Ty -> Prop :=
+Inductive well_scoped_ty (Δ : ctx) : Ty -> Prop :=
   | WST_Var : forall X,
       NameIn X Δ ->
       Δ |-* (Ty_Var X)
@@ -46,17 +41,17 @@ Inductive well_scoped_Ty (Δ : ctx) : Ty -> Prop :=
    *  is this rewrite fine? *)
   | WST_Builtin : forall u (x : typeIn u),
       Δ |-* (Ty_Builtin (@Some' typeIn u x))
-where "Δ '|-*' T " := (well_scoped_Ty Δ T).
+where "Δ '|-*' T " := (well_scoped_ty Δ T).
 
-QCDerive DecOpt for (well_scoped_Ty Δ T).
+QCDerive DecOpt for (well_scoped_ty Δ T).
 
-Instance well_scoped_Ty_DecOpt_sound Δ T : DecOptSoundPos (well_scoped_Ty Δ T).
+Instance well_scoped_ty_DecOpt_sound Δ T : DecOptSoundPos (well_scoped_ty Δ T).
 Proof. Admitted. (* derive_sound. Qed. *)
 
-Instance unique_ty_DecOpt_complete Δ T : DecOptCompletePos (well_scoped_Ty Δ T).
+Instance well_scoped_ty_DecOpt_complete Δ T : DecOptCompletePos (well_scoped_ty Δ T).
 Proof. Admitted. (* derive_complete. Qed. *)
 
-Instance unique_ty_DecOpt_monotonic Δ T: DecOptSizeMonotonic (well_scoped_Ty Δ T).
+Instance well_scoped_ty_DecOpt_monotonic Δ T: DecOptSizeMonotonic (well_scoped_ty Δ T).
 Proof. Admitted. (* derive_mon. Qed. *)
 
 
@@ -64,9 +59,7 @@ Proof. Admitted. (* derive_mon. Qed. *)
 
 Reserved Notation "Δ ',,' Γ '|-+' t " (at level 101, t at level 0, no associativity).
 Reserved Notation "Δ '|-ok_c' c " (at level 101, c at level 0).
-Reserved Notation "Δ ',,' Γ  '|-oks_nr' bs" (at level 101, bs at level 0, no associativity).
-Reserved Notation "Δ ',,' Γ '|-oks_r' bs" (at level 101, bs at level 0, no associativity).
-Reserved Notation "Δ ',,' Γ '|-ok_b' b" (at level 101, b at level 0, no associativity).
+Reserved Notation "Δ '|-ok_cs' cs " (at level 101, cs at level 0).
 
 Inductive constructor_well_formed (Δ : ctx) : constructor -> Prop :=
   | W_Con : forall x T ar,
@@ -77,22 +70,65 @@ Inductive constructor_well_formed (Δ : ctx) : constructor -> Prop :=
 
 QCDerive DecOpt for (constructor_well_formed Δ c).
 
-Instance constructor_well_formed_Ty_DecOpt_sound Δ T : DecOptSoundPos (constructor_well_formed Δ T).
+Instance constructor_well_formed_Ty_DecOpt_sound Δ c : DecOptSoundPos (constructor_well_formed Δ c).
 Proof. Admitted. (* derive_sound. Qed. *)
 
-Instance constructor_well_formed_DecOpt_complete Δ T : DecOptCompletePos (constructor_well_formed Δ T).
+Instance constructor_well_formed_DecOpt_complete Δ c : DecOptCompletePos (constructor_well_formed Δ c).
 Proof. Admitted. (* derive_complete. Qed. *)
 
-Instance constructor_well_formed_DecOpt_monotonic Δ T: DecOptSizeMonotonic (constructor_well_formed Δ T).
+Instance constructor_well_formed_DecOpt_monotonic Δ c : DecOptSizeMonotonic (constructor_well_formed Δ c).
 Proof. Admitted. (* derive_mon. Qed. *)
 
 
 
 
 
-Inductive well_scoped (Δ Γ: ctx) : Term -> Prop :=
+Inductive constructors_well_formed (Δ : ctx) : list constructor -> Prop :=
+  | W_Nil :
+      Δ |-ok_cs nil
+  | W_Cons : forall c cs,
+      Δ |-ok_c c ->
+      Δ |-ok_cs cs ->
+      Δ |-ok_cs (c :: cs)
+  where 
+    "Δ '|-ok_cs' cs" := (constructors_well_formed Δ cs).
+
+QCDerive DecOpt for (constructors_well_formed Δ c).
+
+Instance constructors_well_formed_Ty_DecOpt_sound Δ cs : DecOptSoundPos (constructors_well_formed Δ cs).
+Proof. Admitted. (* derive_sound. Qed. *)
+
+Instance constructors_well_formed_DecOpt_complete Δ cs : DecOptCompletePos (constructors_well_formed Δ cs).
+Proof. Admitted. (* derive_complete. Qed. *)
+
+Instance constructors_well_formed_DecOpt_monotonic Δ cs : DecOptSizeMonotonic (constructors_well_formed Δ cs).
+Proof. Admitted. (* derive_mon. Qed. *)
+
+
+
+
+
+Definition tvd_name (tvd : tvdecl tyname) : tyname :=
+  match tvd with
+  | TyVarDecl v K => v
+  end.
+
+(* Quick cannot hanle function applications with implicit arguments. It ends up generating a function 
+   application, where it tries to non-implicitly apply the implicit argument implicitly... :|.
+   For example: the function application 'rev ls' has as implicit argument the type of the list ls.
+
+   Quick chick would derive an computation that does not do '@rev type ls', but istead does 'rev (@type) ls'
+   which is the exact inverse of what it should do?
+ *)
+Definition rev_map_tvd_name_app YKs Δ := rev (map tvd_name YKs) ++ Δ.
+Definition rev_btvbs_app bs Δ := rev (@btvbs string string bs) ++ Δ.
+Definition rev_bvbs_app bs Γ := rev (@btvbs string string bs) ++ Γ.
+Definition rev_bvbs_data_app c cs bs Γ := rev (rev (map (@bvc string string)  cs) ++ @bvbs string string bs) ++ (c :: Γ).
+Definition rev_bvc_app c cs Γ := c :: (rev (map (@bvc string string) cs)) ++ Γ.
+
+Inductive well_scoped_tm (Δ Γ: ctx) : Term -> Prop :=  
   | WS_Var : forall x,
-      In x Γ ->
+      NameIn x Γ ->
       Δ ,, Γ |-+ (Var x)
   | WS_LamAbs : forall x T t,
       Δ |-* T ->
@@ -117,40 +153,144 @@ Inductive well_scoped (Δ Γ: ctx) : Term -> Prop :=
       Δ ,, Γ |-+ (IWrap F T M)
   | WS_Unwrap : forall M,
       Δ ,, Γ |-+ M ->
-      Δ ,, Γ |-+ (Unwrap M)
-  | WS_Constant : forall u a,
-      Δ ,, Γ |-+ (Constant (Some' (ValueOf u a)))
+      Δ ,, Γ |-+ (Unwrap M) 
+  | WS_Constant : forall u (a : valueOf u),
+      Δ ,, Γ |-+ (Constant (Some' a))
   | WS_Builtin : forall f,
       Δ ,, Γ |-+ (Builtin f)
-  | WS_Error : forall S,
+  (* The original argument 'S' collides with the constructor 'S' in nat*)
+  | WS_Error : forall S',
+      Δ |-* S' ->
+      Δ ,, Γ |-+ (Error S')
+  | WS_Let_NonRec_Nil : forall t,
+      Δ ,, Γ |-+ t ->
+      Δ ,, Γ |-+ (Let NonRec nil t)
+  | WS_Let_NonRec_TermBind : forall bs t t' s x T,
+      Δ |-* T ->
+      Δ ,, Γ |-+ t' ->
+      rev_btvbs_app bs Δ ,, rev_btvbs_app bs (x :: Γ) |-+ t ->
+      (* The term 't' only needs to be checked once here. The constant is a hack to be able to check the
+       * bindings in bs, without causing further checks of 't', and a constant is always well-bounded *)
+      Δ ,, Γ |-+ (Let Rec bs (Constant (Some' (ValueOf DefaultUniBool true)))) ->
+      Δ ,, Γ |-+ (Let NonRec ((TermBind s (VarDecl x T) t') :: bs) t)
+  | WS_Let_NonRec_TypeBind : forall bs t X K T,
+      Δ |-* T ->
+      rev_btvbs_app bs (X :: Δ) ,, rev_bvbs_app bs Γ |-+ t ->
+      (* The term 't' only needs to be checked once here. The constant is a hack to be able to check the
+       * bindings in bs, without causing further checks of 't', and a constant is always well-bounded *)
+      Δ ,, Γ |-+ (Let Rec bs (Constant (Some' (ValueOf DefaultUniBool true)))) ->
+      Δ ,, Γ |-+ (Let NonRec ((TypeBind (TyVarDecl X K) T) :: bs) t)
+  | WS_Let_NonRec_DatatypeBind : forall bs t X K YKs c cs,
+      constructors_well_formed (rev_map_tvd_name_app YKs Δ) cs ->
+      rev_btvbs_app bs (X :: Δ) ,, rev_bvbs_data_app c cs bs Γ |-+ t ->
+      (* The term 't' only needs to be checked once here. The constant is a hack to be able to check the
+       * bindings in bs, without causing further checks of 't', and a constant is always well-bounded *)
+      Δ ,, Γ |-+ (Let Rec bs (Constant (Some' (ValueOf DefaultUniBool true)))) ->
+      Δ ,, Γ |-+ (Let NonRec ((DatatypeBind (Datatype (TyVarDecl X K) YKs c cs)) :: bs) t)
+  | WS_Let_Rec_Nil : forall t,
+      Δ ,, Γ |-+ t ->
+      Δ ,, Γ |-+ (Let Rec nil t)
+  | WS_Let_Rec_TermBind : forall bs t t' s x T,
+      Δ |-* T ->
+      Δ ,, Γ |-+ t' ->
+      Δ ,, (x :: Γ) |-+ (Let NonRec bs t) ->
+      Δ ,, Γ |-+ (Let Rec ((TermBind s (VarDecl x T) t') :: bs) t)
+  | WS_Let_Rec_TypeBind : forall bs t X K T,
+      Δ |-* T ->
+      (X :: Δ) ,, Γ |-+ (Let NonRec bs t) ->
+      Δ ,, Γ |-+ (Let Rec ((TypeBind (TyVarDecl X K) T) :: bs) t)
+  | WS_Let_Rec_DatabindType : forall bs t X K YKs c cs,
+      constructors_well_formed (rev_map_tvd_name_app YKs Δ) cs ->
+      (X :: Δ) ,, rev_bvc_app c cs Γ |-+ (Let NonRec bs t) ->
+      Δ ,, Γ |-+ (Let Rec ((DatatypeBind (Datatype (TyVarDecl X K) YKs c cs)) :: bs) t) 
+  where "Δ ',,' Γ '|-+' t" := (well_scoped_tm Δ Γ t).
+           
+(*
+ * (rev (btvbs bs) ++ Δ) ,, (rev (bvbs bs) ++ (x :: Γ)) |-+ t
+ *
+ * let unkn_1859_ := btvbs (@string) (@string) bs in
+ * let unkn_1860_ := rev (@string) unkn_1859_ in
+ * let unkn_1861_ := app (@string) unkn_1860_ Δ_ in
+ * let unkn_1862_ := bvbs (@string) (@string) bs in
+ * let unkn_1863_ := rev (@string) unkn_1862_
+ *)
+
+QCDerive DecOpt for (well_scoped_tm Δ Γ tm).
+
+Instance well_scoped_tm_DecOpt_sound Δ Γ tm : DecOptSoundPos (well_scoped_tm Δ Γ tm).
+Proof. Admitted. (* derive_sound. Qed. *)
+
+Instance well_scoped_tm_DecOpt_complete Δ Γ tm : DecOptCompletePos (well_scoped_tm Δ Γ tm).
+Proof. Admitted. (* derive_complete. Qed. *)
+
+Instance well_scoped_tm_DecOpt_monotonic Δ Γ tm: DecOptSizeMonotonic (well_scoped_tm Δ Γ tm).
+Proof. Admitted. (* derive_mon. Qed. *)
+
+(* Original well_scoped definition, including mutual recursion *)
+
+Reserved Notation "Δ ',,' Γ '|-old' t " (at level 101, t at level 0, no associativity).
+Reserved Notation "Δ ',,' Γ '|-oks_nr' bs" (at level 101, bs at level 0, no associativity).
+Reserved Notation "Δ ',,' Γ '|-oks_r' bs" (at level 101, bs at level 0, no associativity).
+Reserved Notation "Δ ',,' Γ '|-ok_b' b" (at level 101, b at level 0, no associativity).
+
+
+Inductive well_scoped_old (Δ Γ: ctx) : Term -> Prop :=
+  | WS_Var' : forall x,
+      In x Γ ->
+      Δ ,, Γ |-old (Var x)
+  | WS_LamAbs' : forall x T t,
+      Δ |-* T ->
+      Δ ,, (x :: Γ) |-old t ->
+      Δ ,, Γ |-old (LamAbs x T t)
+  | WS_Apply' : forall t1 t2,
+      Δ ,, Γ |-old t1 ->
+      Δ ,, Γ |-old t2 ->
+      Δ ,, Γ |-old (Apply t1 t2)
+  (* Universal types *)
+  | WS_TyAbs' : forall X K t,
+      (X :: Δ) ,, Γ |-old t ->
+      Δ ,, Γ |-old (TyAbs X K t)
+  | WS_TyInst' : forall t T,
+      Δ ,, Γ |-old t ->
+      Δ |-* T ->
+      Δ ,, Γ |-old (TyInst t T)
+  | WS_IWrap' : forall F T M,
+      Δ |-* F ->
+      Δ |-* T ->
+      Δ ,, Γ |-old M ->
+      Δ ,, Γ |-old (IWrap F T M)
+  | WS_Unwrap' : forall M,
+      Δ ,, Γ |-old M ->
+      Δ ,, Γ |-old (Unwrap M)
+  | WS_Constant' : forall u a,
+      Δ ,, Γ |-old (Constant (Some' (ValueOf u a)))
+  | WS_Builtin' : forall f,
+      Δ ,, Γ |-old (Builtin f)
+  | WS_Error' : forall S,
       Δ |-* S ->
-      Δ ,, Γ |-+ (Error S)
-  | WS_Let : forall bs t Δ' Γ',
+      Δ ,, Γ |-old (Error S)
+  | WS_Let' : forall bs t Δ' Γ',
       Δ' = rev (btvbs bs) ++ Δ ->
       Γ' = rev (bvbs bs) ++ Γ ->
       Δ ,, Γ |-oks_nr bs ->
-      Δ' ,, Γ' |-+ t ->
-      Δ ,, Γ |-+ (Let NonRec bs t)
-  | WS_LetRec : forall bs t Δ' Γ',
+      Δ' ,, Γ' |-old t ->
+      Δ ,, Γ |-old (Let NonRec bs t)
+  | WS_LetRec' : forall bs t Δ' Γ',
       Δ' = rev (btvbs bs) ++ Δ ->
       Γ' = rev (bvbs bs) ++ Γ ->
       Δ' ,, Γ' |-oks_r bs ->
-      Δ' ,, Γ' |-+ t ->
-      Δ ,, Γ |-+ (Let Rec bs t)
-
+      Δ' ,, Γ' |-old t ->
+      Δ ,, Γ |-old (Let Rec bs t)
 
 with bindings_well_formed_nonrec (Δ Γ : ctx) : list Binding -> Prop :=
-
   | W_NilB_NonRec :
     Δ ,, Γ |-oks_nr nil
-
   | W_ConsB_NonRec : forall b bs,
       Δ ,, Γ |-ok_b b ->
       (btvb b ++ Δ) ,, (bvb b ++ Γ) |-oks_nr bs ->
       Δ ,, Γ |-oks_nr (b :: bs)
 
 with bindings_well_formed_rec (Δ Γ : ctx) : list Binding -> Prop :=
-
   | W_NilB_Rec :
       Δ ,, Γ |-oks_r nil
   | W_ConsB_Rec : forall b bs,
@@ -161,7 +301,7 @@ with bindings_well_formed_rec (Δ Γ : ctx) : list Binding -> Prop :=
 with binding_well_formed (Δ Γ : ctx) : Binding -> Prop :=
   | W_Term : forall s x T t,
       Δ |-* T ->
-      Δ ,, Γ |-+ t ->
+      Δ ,, Γ |-old t ->
       Δ ,, Γ |-ok_b (TermBind s (VarDecl x T) t)
   | W_Type : forall X K T,
       Δ |-* T ->
@@ -171,8 +311,22 @@ with binding_well_formed (Δ Γ : ctx) : Binding -> Prop :=
       (forall c, In c cs -> Δ' |-ok_c c) ->
       Δ ,, Γ |-ok_b (DatatypeBind (Datatype X YKs matchFunc cs))
 
-  where "Δ ',,' Γ '|-+' t" := (well_scoped Δ Γ t)
+  where "Δ ',,' Γ '|-old' t" := (well_scoped_old Δ Γ t)
   and "Δ ',,' Γ '|-oks_nr' bs" := (bindings_well_formed_nonrec Δ Γ bs)
   and "Δ ',,' Γ '|-oks_r' bs" := (bindings_well_formed_rec Δ Γ bs)
-  and "Δ ',,' Γ '|-ok_b' b" := (binding_well_formed Δ Γ b)
-.
+  and "Δ ',,' Γ '|-ok_b' b" := (binding_well_formed Δ Γ b).
+
+(* TODO: not finished, but is this necessary? *)
+Lemma well_scoped_eq : forall Δ Γ tm,
+  well_scoped_tm Δ Γ tm <-> well_scoped_old Δ Γ tm.
+Proof.
+  intros Δ Γ tm; split; revert Δ Γ.
+  - induction tm; intros;
+    try (inversion H; constructor; try apply NameIn_In_string_equal; try apply IHtm1; try apply IHtm2; try apply IHtm; assumption; reflexivity).
+    + admit.
+    + inversion H; induction a; constructor. 
+  - induction tm; intros;
+    try (inversion H; constructor; try apply IHtm; try apply IHtm1; try apply IHtm2; assumption; reflexivity).
+    + admit.
+    + constructor. inversion H. apply NameIn_In_string_equal. apply H1.
+Admitted.
